Define used PID in the sequential setup

src/Concurrent/PIDRenaming.v
@@ -2,105 +2,105 @@ From CoreErlang.FrameStack Require Import SubstSemanticsLemmas.
 
 Import ListNotations.
 
-Fixpoint rename_PID (from to : PID) (e : Exp) : Exp :=
+Fixpoint renamePID (from to : PID) (e : Exp) : Exp :=
 match e with
- | VVal e => VVal (rename_PID_val from to e)
- | EExp e => EExp (rename_PID_nval from to e)
+ | VVal e => VVal (renamePIDVal from to e)
+ | EExp e => EExp (renamePIDNVal from to e)
 end
-with rename_PID_val (from to : PID) (v : Val) : Val :=
+with renamePIDVal (from to : PID) (v : Val) : Val :=
 match v with
  | VNil => VNil
  | VLit l => VLit l
  | VPid p =>
    if Nat.eqb from p then VPid to else VPid p
- | VCons hd tl => VCons (rename_PID_val from to hd) (rename_PID_val from to tl)
- | VTuple l => VTuple (map (rename_PID_val from to) l)
- | VMap l => VMap (map (fun '(x,y) => (rename_PID_val from to x, rename_PID_val from to y)) l)
+ | VCons hd tl => VCons (renamePIDVal from to hd) (renamePIDVal from to tl)
+ | VTuple l => VTuple (map (renamePIDVal from to) l)
+ | VMap l => VMap (map (fun '(x,y) => (renamePIDVal from to x, renamePIDVal from to y)) l)
  | VVar n => VVar n
  | VFunId n => VFunId n
- | VClos ext id params e => VClos (map (fun '(id, vl, e) => (id, vl, rename_PID from to e)) ext) id params (rename_PID from to e)
+ | VClos ext id params e => VClos (map (fun '(id, vl, e) => (id, vl, renamePID from to e)) ext) id params (renamePID from to e)
 end
-with rename_PID_nval (from to : PID) (n : NonVal) : NonVal :=
+with renamePIDNVal (from to : PID) (n : NonVal) : NonVal :=
 match n with
- | EFun vl e => EFun vl (rename_PID from to e)
- | EValues el => EValues (map (rename_PID from to) el)
- | ECons hd tl => ECons (rename_PID from to hd) (rename_PID from to tl)
- | ETuple l => ETuple (map (rename_PID from to) l)
- | EMap l => EMap (map (fun '(x,y) => (rename_PID from to x, rename_PID from to y)) l)
- | ECall m f l => ECall (rename_PID from to m) (rename_PID from to f) (map (rename_PID from to) l)
- | EPrimOp f l => EPrimOp f (map (rename_PID from to) l)
- | EApp exp l => EApp (rename_PID from to exp) (map (rename_PID from to) l)
- | ECase e l => ECase (rename_PID from to e)
-                      (map (fun '(p, g, e) => (p, rename_PID from to g, rename_PID from to e)) l)
- | ELet l e1 e2 => ELet l (rename_PID from to e1) (rename_PID from to e2)
- | ESeq e1 e2 => ESeq (rename_PID from to e1) (rename_PID from to e2)
- | ELetRec l e => ELetRec (map (fun '(vl, e) => (vl, rename_PID from to e)) l)
-                          (rename_PID from to e)
- | ETry e1 vl1 e2 vl2 e3 => ETry (rename_PID from to e1)
-                                 vl1 (rename_PID from to e2)
-                                 vl2 (rename_PID from to e3)
+ | EFun vl e => EFun vl (renamePID from to e)
+ | EValues el => EValues (map (renamePID from to) el)
+ | ECons hd tl => ECons (renamePID from to hd) (renamePID from to tl)
+ | ETuple l => ETuple (map (renamePID from to) l)
+ | EMap l => EMap (map (fun '(x,y) => (renamePID from to x, renamePID from to y)) l)
+ | ECall m f l => ECall (renamePID from to m) (renamePID from to f) (map (renamePID from to) l)
+ | EPrimOp f l => EPrimOp f (map (renamePID from to) l)
+ | EApp exp l => EApp (renamePID from to exp) (map (renamePID from to) l)
+ | ECase e l => ECase (renamePID from to e)
+                      (map (fun '(p, g, e) => (p, renamePID from to g, renamePID from to e)) l)
+ | ELet l e1 e2 => ELet l (renamePID from to e1) (renamePID from to e2)
+ | ESeq e1 e2 => ESeq (renamePID from to e1) (renamePID from to e2)
+ | ELetRec l e => ELetRec (map (fun '(vl, e) => (vl, renamePID from to e)) l)
+                          (renamePID from to e)
+ | ETry e1 vl1 e2 vl2 e3 => ETry (renamePID from to e1)
+                                 vl1 (renamePID from to e2)
+                                 vl2 (renamePID from to e3)
 end.
 
-Notation "e .[ x ↦ y ]" := (rename_PID x y e) (at level 2).
-Notation "e .[ x ↦ y ]ᵥ" := (rename_PID_val x y e) (at level 2).
-Notation "e .[ x ↦ y ]ₙ" := (rename_PID_nval x y e) (at level 2).
+Notation "e .[ x ↦ y ]" := (renamePID x y e) (at level 2).
+Notation "e .[ x ↦ y ]ᵥ" := (renamePIDVal x y e) (at level 2).
+Notation "e .[ x ↦ y ]ₙ" := (renamePIDNVal x y e) (at level 2).
 
-Definition rename_PID_red (from to : PID) (r : Redex) : Redex :=
+Definition renamePIDRed (from to : PID) (r : Redex) : Redex :=
 match r with
- | RExp e => RExp (rename_PID from to e)
- | RValSeq vs => RValSeq (map (rename_PID_val from to) vs)
- | RExc (class, reas, det) => RExc (class, rename_PID_val from to reas,
-                                           rename_PID_val from to det)
+ | RExp e => RExp (renamePID from to e)
+ | RValSeq vs => RValSeq (map (renamePIDVal from to) vs)
+ | RExc (class, reas, det) => RExc (class, renamePIDVal from to reas,
+                                           renamePIDVal from to det)
  | RBox => RBox
 end.
 
-Notation "e .[ x ↦ y ]ᵣ" := (rename_PID_red x y e) (at level 2).
+Notation "e .[ x ↦ y ]ᵣ" := (renamePIDRed x y e) (at level 2).
 
-Definition rename_PID_frameId (from to : PID) (f : FrameIdent) : FrameIdent :=
+Definition renamePIDFrameId (from to : PID) (f : FrameIdent) : FrameIdent :=
 match f with
  | IValues => f
  | ITuple => f
  | IMap => f
- | ICall m f => ICall (rename_PID_val from to m) (rename_PID_val from to f)
+ | ICall m f => ICall (renamePIDVal from to m) (renamePIDVal from to f)
  | IPrimOp f => IPrimOp f
- | IApp v => IApp (rename_PID_val from to v)
+ | IApp v => IApp (renamePIDVal from to v)
 end.
 
-Notation "e .[ x ↦ y ]ᵢ" := (rename_PID_frameId x y e) (at level 2).
+Notation "e .[ x ↦ y ]ᵢ" := (renamePIDFrameId x y e) (at level 2).
 
-Definition rename_PID_frame (from to : PID) (f : Frame) : Frame :=
+Definition renamePIDFrame (from to : PID) (f : Frame) : Frame :=
 match f with
- | FCons1 hd => FCons1 (rename_PID from to hd)
- | FCons2 tl => FCons2 (rename_PID_val from to tl)
+ | FCons1 hd => FCons1 (renamePID from to hd)
+ | FCons2 tl => FCons2 (renamePIDVal from to tl)
  | FParams ident vl el =>
-     FParams (rename_PID_frameId from to ident) (map (rename_PID_val from to) vl)
-                                                (map (rename_PID from to) el)
- | FApp1 l => FApp1 (map (rename_PID from to) l)
- | FCallMod f l => FCallMod (rename_PID from to f) (map (rename_PID from to) l)
- | FCallFun m l => FCallFun (rename_PID_val from to m) (map (rename_PID from to) l)
- | FCase1 l => FCase1 (map (fun '(p, g, e) => (p, rename_PID from to g, rename_PID from to e)) l)
+     FParams (renamePIDFrameId from to ident) (map (renamePIDVal from to) vl)
+                                                (map (renamePID from to) el)
+ | FApp1 l => FApp1 (map (renamePID from to) l)
+ | FCallMod f l => FCallMod (renamePID from to f) (map (renamePID from to) l)
+ | FCallFun m l => FCallFun (renamePIDVal from to m) (map (renamePID from to) l)
+ | FCase1 l => FCase1 (map (fun '(p, g, e) => (p, renamePID from to g, renamePID from to e)) l)
  | FCase2 lv ex le =>
    FCase2
-     (map (rename_PID_val from to) lv)
-     (rename_PID from to ex)
-     (map (fun '(p, g, e) => (p, rename_PID from to g, rename_PID from to e)) le)
- | FLet l e => FLet l (rename_PID from to e)
- | FSeq e => FSeq (rename_PID from to e)
- | FTry vl1 e2 vl2 e3 => FTry vl1 (rename_PID from to e2)
-                              vl2 (rename_PID from to e3)
+     (map (renamePIDVal from to) lv)
+     (renamePID from to ex)
+     (map (fun '(p, g, e) => (p, renamePID from to g, renamePID from to e)) le)
+ | FLet l e => FLet l (renamePID from to e)
+ | FSeq e => FSeq (renamePID from to e)
+ | FTry vl1 e2 vl2 e3 => FTry vl1 (renamePID from to e2)
+                              vl2 (renamePID from to e3)
 end.
 
-Notation "e .[ x ↦ y ]ₖ" := (rename_PID_frame x y e) (at level 2).
+Notation "e .[ x ↦ y ]ₖ" := (renamePIDFrame x y e) (at level 2).
 
-Definition rename_PID_stack (from to : PID) (fs : FrameStack) :=
-  map (rename_PID_frame from to) fs.
+Definition renamePIDStack (from to : PID) (fs : FrameStack) :=
+  map (renamePIDFrame from to) fs.
 
-Notation "e .[ x ↦ y ]ₛ" := (rename_PID_stack x y e) (at level 2).
+Notation "e .[ x ↦ y ]ₛ" := (renamePIDStack x y e) (at level 2).
 
-Lemma rename_PID_preserves_scope :
-  (forall Γ e, EXP Γ ⊢ e -> forall from to, EXP Γ ⊢ rename_PID from to e) /\
-  (forall Γ e, VAL Γ ⊢ e -> forall from to, VAL Γ ⊢ rename_PID_val from to e) /\
-  (forall Γ e, NVAL Γ ⊢ e -> forall from to, NVAL Γ ⊢ rename_PID_nval from to e).
+Lemma renamePID_preserves_scope :
+  (forall Γ e, EXP Γ ⊢ e -> forall from to, EXP Γ ⊢ renamePID from to e) /\
+  (forall Γ e, VAL Γ ⊢ e -> forall from to, VAL Γ ⊢ renamePIDVal from to e) /\
+  (forall Γ e, NVAL Γ ⊢ e -> forall from to, NVAL Γ ⊢ renamePIDNVal from to e).
 Proof.
   apply scoped_ind; intros; cbn; try now constructor.
   * break_match_goal; constructor.
@@ -168,7 +168,7 @@ Proof.
              (fst ∘ fst)
                (let
                 '(p, g, e3) := x in
-                 (p, rename_PID from to g, rename_PID from to e3)))) (d := ([], `VNil, `VNil)).
+                 (p, renamePID from to g, renamePID from to e3)))) (d := ([], `VNil, `VNil)).
       rewrite map_length in H2. eapply H0 in H2.
       rewrite map_nth with (d := ([], `VNil, `VNil)) in H2.
       setoid_rewrite (map_nth (fst ∘ fst)) with (d := ([], `VNil, `VNil)) in H2.
@@ -179,7 +179,7 @@ Proof.
              (fst ∘ fst)
                (let
                 '(p, g, e3) := x in
-                 (p, rename_PID from to g, rename_PID from to e3)))) (d := ([], `VNil, `VNil)).
+                 (p, renamePID from to g, renamePID from to e3)))) (d := ([], `VNil, `VNil)).
       rewrite map_length in H2. eapply H1 in H2.
       rewrite map_nth with (d := ([], `VNil, `VNil)) in H2.
       setoid_rewrite (map_nth (fst ∘ fst)) with (d := ([], `VNil, `VNil)) in H2.
@@ -193,44 +193,44 @@ Proof.
     - rewrite map_length. apply H0.
 Qed.
 
-Definition rename_PID_subst (from to : PID) (σ : Substitution) : Substitution :=
+Definition renamePID_subst (from to : PID) (σ : Substitution) : Substitution :=
   fun x =>
     match σ x with
-    | inl val => inl (rename_PID_val from to val)
+    | inl val => inl (renamePIDVal from to val)
     | r => r
     end.
 
-Theorem rename_rename_PID :
-  (forall e ρ from to, rename ρ (rename_PID from to e) =
-                      rename_PID from to (rename ρ e)) /\
-  (forall e ρ from to, renameNonVal ρ (rename_PID_nval from to e) =
-                      rename_PID_nval from to (renameNonVal ρ e)) /\
-  (forall e ρ from to, renameVal ρ (rename_PID_val from to e) =
-                      rename_PID_val from to (renameVal ρ e)).
+Theorem rename_renamePID :
+  (forall e ρ from to, rename ρ (renamePID from to e) =
+                      renamePID from to (rename ρ e)) /\
+  (forall e ρ from to, renameNonVal ρ (renamePIDNVal from to e) =
+                      renamePIDNVal from to (renameNonVal ρ e)) /\
+  (forall e ρ from to, renameVal ρ (renamePIDVal from to e) =
+                      renamePIDVal from to (renameVal ρ e)).
 Proof.
   eapply Exp_ind with
-    (QV := fun l => Forall (fun e => forall ρ from to, renameVal ρ (rename_PID_val from to e) =
-                      rename_PID_val from to (renameVal ρ e)) l)
-    (Q := fun l => Forall (fun e => forall ρ from to, rename ρ (rename_PID from to e) =
-                      rename_PID from to (rename ρ e)) l)
-    (RV := fun l => Forall (fun '(e1, e2) => forall ρ from to, renameVal ρ (rename_PID_val from to e1) =
-                      rename_PID_val from to (renameVal ρ e1) /\
-         renameVal ρ (rename_PID_val from to e2) =
-                      rename_PID_val from to (renameVal ρ e2)) l)
-    (R := fun l => Forall (fun '(e1, e2) => forall from to ρ, rename ρ (rename_PID from to e1) =
-                      rename_PID from to (rename ρ e1) /\
-         rename ρ (rename_PID from to e2) =
-                      rename_PID from to (rename ρ e2)) l)
+    (QV := fun l => Forall (fun e => forall ρ from to, renameVal ρ (renamePIDVal from to e) =
+                      renamePIDVal from to (renameVal ρ e)) l)
+    (Q := fun l => Forall (fun e => forall ρ from to, rename ρ (renamePID from to e) =
+                      renamePID from to (rename ρ e)) l)
+    (RV := fun l => Forall (fun '(e1, e2) => forall ρ from to, renameVal ρ (renamePIDVal from to e1) =
+                      renamePIDVal from to (renameVal ρ e1) /\
+         renameVal ρ (renamePIDVal from to e2) =
+                      renamePIDVal from to (renameVal ρ e2)) l)
+    (R := fun l => Forall (fun '(e1, e2) => forall from to ρ, rename ρ (renamePID from to e1) =
+                      renamePID from to (rename ρ e1) /\
+         rename ρ (renamePID from to e2) =
+                      renamePID from to (rename ρ e2)) l)
     (W := fun l => Forall (fun '(p, g, e) => forall from to ρ,
-       rename ρ (rename_PID from to g) =
-                      rename_PID from to (rename ρ g) /\
-       rename ρ (rename_PID from to e) =
-                      rename_PID from to (rename ρ e)) l)
-    (Z := fun l => Forall (fun '(n, e) => forall from to ρ, rename ρ (rename_PID from to e) =
-                      rename_PID from to (rename ρ e)) l)
+       rename ρ (renamePID from to g) =
+                      renamePID from to (rename ρ g) /\
+       rename ρ (renamePID from to e) =
+                      renamePID from to (rename ρ e)) l)
+    (Z := fun l => Forall (fun '(n, e) => forall from to ρ, rename ρ (renamePID from to e) =
+                      renamePID from to (rename ρ e)) l)
    (VV := fun l => Forall
-      (fun '(id, vl, e) => forall from to ρ, rename ρ (rename_PID from to e) =
-                      rename_PID from to (rename ρ e)) l)
+      (fun '(id, vl, e) => forall from to ρ, rename ρ (renamePID from to e) =
+                      renamePID from to (rename ρ e)) l)
   ; intros.
   all: cbn; auto.
   1-2: now rewrite H.
@@ -282,55 +282,55 @@ Proof.
   * now rewrite H, H0, H1.
 Qed.
 
-Lemma rename_PID_subst_up :
-  forall σ from to, up_subst (rename_PID_subst from to σ) =
-                    rename_PID_subst from to (up_subst σ).
+Lemma renamePID_subst_up :
+  forall σ from to, up_subst (renamePID_subst from to σ) =
+                    renamePID_subst from to (up_subst σ).
 Proof.
-  unfold rename_PID_subst, up_subst. intros.
+  unfold renamePID_subst, up_subst. intros.
   extensionality x. destruct x; auto.
   unfold shift. destruct σ; auto.
-  now rewrite (proj2 (proj2 rename_rename_PID)).
+  now rewrite (proj2 (proj2 rename_renamePID)).
 Qed.
 
-Corollary rename_PID_upn :
-  forall n σ from to, upn n (rename_PID_subst from to σ) =
-                      rename_PID_subst from to (upn n σ).
+Corollary renamePID_upn :
+  forall n σ from to, upn n (renamePID_subst from to σ) =
+                      renamePID_subst from to (upn n σ).
 Proof.
   induction n; intros; simpl; auto.
-  now rewrite IHn, rename_PID_subst_up.
+  now rewrite IHn, renamePID_subst_up.
 Qed.
 
-Theorem split_rename_PID_subst :
-     (forall e from to σ, rename_PID from to e.[σ] = 
-       (rename_PID from to e).[rename_PID_subst from to σ])
-  /\ (forall e from to σ, rename_PID_nval from to e.[σ]ₑ = 
-       (rename_PID_nval from to e).[rename_PID_subst from to σ]ₑ)
-  /\ (forall e from to σ, rename_PID_val from to e.[σ]ᵥ = 
-       (rename_PID_val from to e).[rename_PID_subst from to σ]ᵥ).
+Theorem split_renamePID_subst :
+     (forall e from to σ, renamePID from to e.[σ] = 
+       (renamePID from to e).[renamePID_subst from to σ])
+  /\ (forall e from to σ, renamePIDNVal from to e.[σ]ₑ = 
+       (renamePIDNVal from to e).[renamePID_subst from to σ]ₑ)
+  /\ (forall e from to σ, renamePIDVal from to e.[σ]ᵥ = 
+       (renamePIDVal from to e).[renamePID_subst from to σ]ᵥ).
 Proof.
   eapply Exp_ind with
-    (QV := fun l => Forall (fun e => forall from to σ, rename_PID_val from to e.[σ]ᵥ = 
-       (rename_PID_val from to e).[rename_PID_subst from to σ]ᵥ) l)
-    (Q := fun l => Forall (fun e => forall from to σ, rename_PID from to e.[σ] = 
-       (rename_PID from to e).[rename_PID_subst from to σ]) l)
-    (RV := fun l => Forall (fun '(e1, e2) => forall from to σ, rename_PID_val from to e1.[σ]ᵥ = 
-       (rename_PID_val from to e1).[rename_PID_subst from to σ]ᵥ /\
-         rename_PID_val from to e2.[σ]ᵥ = 
-       (rename_PID_val from to e2).[rename_PID_subst from to σ]ᵥ) l)
-    (R := fun l => Forall (fun '(e1, e2) => forall from to σ, rename_PID from to e1.[σ] = 
-       (rename_PID from to e1).[rename_PID_subst from to σ] /\
-         rename_PID from to e2.[σ] = 
-       (rename_PID from to e2).[rename_PID_subst from to σ]) l)
+    (QV := fun l => Forall (fun e => forall from to σ, renamePIDVal from to e.[σ]ᵥ = 
+       (renamePIDVal from to e).[renamePID_subst from to σ]ᵥ) l)
+    (Q := fun l => Forall (fun e => forall from to σ, renamePID from to e.[σ] = 
+       (renamePID from to e).[renamePID_subst from to σ]) l)
+    (RV := fun l => Forall (fun '(e1, e2) => forall from to σ, renamePIDVal from to e1.[σ]ᵥ = 
+       (renamePIDVal from to e1).[renamePID_subst from to σ]ᵥ /\
+         renamePIDVal from to e2.[σ]ᵥ = 
+       (renamePIDVal from to e2).[renamePID_subst from to σ]ᵥ) l)
+    (R := fun l => Forall (fun '(e1, e2) => forall from to σ, renamePID from to e1.[σ] = 
+       (renamePID from to e1).[renamePID_subst from to σ] /\
+         renamePID from to e2.[σ] = 
+       (renamePID from to e2).[renamePID_subst from to σ]) l)
     (W := fun l => Forall (fun '(p, g, e) => forall from to σ,
-       rename_PID from to g.[σ] =
-       (rename_PID from to g).[(rename_PID_subst from to σ)] /\
-       rename_PID from to e.[σ] = 
-       (rename_PID from to e).[(rename_PID_subst from to σ)]) l)
-    (Z := fun l => Forall (fun '(n, e) => forall from to σ, rename_PID from to e.[σ] = 
-       (rename_PID from to e).[(rename_PID_subst from to σ)]) l)
+       renamePID from to g.[σ] =
+       (renamePID from to g).[(renamePID_subst from to σ)] /\
+       renamePID from to e.[σ] = 
+       (renamePID from to e).[(renamePID_subst from to σ)]) l)
+    (Z := fun l => Forall (fun '(n, e) => forall from to σ, renamePID from to e.[σ] = 
+       (renamePID from to e).[(renamePID_subst from to σ)]) l)
    (VV := fun l => Forall
-      (fun '(id, vl, e) => forall from to σ, rename_PID from to e.[σ] = 
-       (rename_PID from to e).[(rename_PID_subst from to σ)]) l)
+      (fun '(id, vl, e) => forall from to σ, renamePID from to e.[σ] = 
+       (renamePID from to e).[(renamePID_subst from to σ)]) l)
   ; intros.
   all: cbn; auto.
   1-2: now rewrite H.
@@ -341,14 +341,14 @@ Proof.
   * f_equal. do 2 rewrite map_map. apply map_ext_Forall.
     induction H; constructor; auto. destruct x.
     specialize (H from to σ) as [H_1 H_2]. now rewrite H_1, H_2.
-  * unfold rename_PID_subst. now destruct σ.
-  * unfold rename_PID_subst. destruct n. now destruct σ.
+  * unfold renamePID_subst. now destruct σ.
+  * unfold renamePID_subst. destruct n. now destruct σ.
   * f_equal.
     - do 2 rewrite map_map. apply map_ext_Forall.
       rewrite Forall_nth in *. intros. eapply (H _ d) in H1. destruct nth, p.
-      rewrite H1. now rewrite map_length, rename_PID_upn.
-    - rewrite map_length. now rewrite H0, rename_PID_upn.
-  * now rewrite H, rename_PID_upn.
+      rewrite H1. now rewrite map_length, renamePID_upn.
+    - rewrite map_length. now rewrite H0, renamePID_upn.
+  * now rewrite H, renamePID_upn.
   * f_equal. do 2 rewrite map_map. apply map_ext_Forall.
     induction H; constructor; auto.
   * now rewrite H, H0.
@@ -372,51 +372,51 @@ Proof.
     - now rewrite H.
     - do 2 rewrite map_map. apply map_ext_Forall.
       rewrite Forall_nth in *. intros. eapply (H0 _ d) in H1. destruct nth, p.
-      rewrite (proj1 (H1 _ _ _)), (proj2 (H1 _ _ _)). now rewrite rename_PID_upn.
-  * rewrite H, H0. now rewrite rename_PID_upn.
+      rewrite (proj1 (H1 _ _ _)), (proj2 (H1 _ _ _)). now rewrite renamePID_upn.
+  * rewrite H, H0. now rewrite renamePID_upn.
   * now rewrite H, H0.
   * f_equal.
     - do 2 rewrite map_map. apply map_ext_Forall.
       rewrite Forall_nth in *. intros. eapply (H0 _ d) in H1. destruct nth.
-      rewrite (H1 _ _ _). now rewrite rename_PID_upn, map_length.
-    - rewrite H. now rewrite map_length, rename_PID_upn.
-  * rewrite H, H0, H1. now repeat rewrite rename_PID_upn.
+      rewrite (H1 _ _ _). now rewrite renamePID_upn, map_length.
+    - rewrite H. now rewrite map_length, renamePID_upn.
+  * rewrite H, H0, H1. now repeat rewrite renamePID_upn.
 Qed.
 
-Corollary split_rename_PID_subst_exp :
-  (forall e from to σ, rename_PID from to e.[σ] = 
-    (rename_PID from to e).[rename_PID_subst from to σ]).
+Corollary split_renamePID_subst_exp :
+  (forall e from to σ, renamePID from to e.[σ] = 
+    (renamePID from to e).[renamePID_subst from to σ]).
 Proof.
-  apply split_rename_PID_subst.
+  apply split_renamePID_subst.
 Qed.
 
-Corollary split_rename_PID_subst_val :
-  (forall e from to σ, rename_PID_val from to e.[σ]ᵥ = 
-       (rename_PID_val from to e).[rename_PID_subst from to σ]ᵥ).
+Corollary split_renamePID_subst_val :
+  (forall e from to σ, renamePIDVal from to e.[σ]ᵥ = 
+       (renamePIDVal from to e).[renamePID_subst from to σ]ᵥ).
 Proof.
-  apply split_rename_PID_subst.
+  apply split_renamePID_subst.
 Qed.
 
-Proposition rename_PID_subst_id :
-  forall from to, rename_PID_subst from to idsubst = idsubst.
+Proposition renamePID_subst_id :
+  forall from to, renamePID_subst from to idsubst = idsubst.
 Proof.
   now intros.
 Qed.
 
-Proposition rename_PID_subst_list_subst :
+Proposition renamePID_subst_list_subst :
   forall vs from to σ,
-    rename_PID_subst from to (list_subst vs σ) =
-    list_subst (map (rename_PID_val from to) vs) (rename_PID_subst from to σ).
+    renamePID_subst from to (list_subst vs σ) =
+    list_subst (map (renamePIDVal from to) vs) (renamePID_subst from to σ).
 Proof.
   induction vs; simpl; intros; auto.
-  rewrite <- IHvs. clear. unfold scons, rename_PID_subst.
+  rewrite <- IHvs. clear. unfold scons, renamePID_subst.
   extensionality x. destruct x; auto.
 Qed.
 
 Proposition rename_subst_flatten_list :
   forall el from to, 
-    map (rename_PID from to) (flatten_list el) =
-    flatten_list (map (fun '(x, y) => (rename_PID from to x, rename_PID from to y)) el).
+    map (renamePID from to) (flatten_list el) =
+    flatten_list (map (fun '(x, y) => (renamePID from to x, renamePID from to y)) el).
 Proof.
   induction el using list_length_ind; destruct el; intros; simpl; auto.
   destruct p. simpl. do 2 f_equal. rewrite H. reflexivity. slia.
@@ -424,26 +424,26 @@ Qed.
 
 Proposition rename_subst_deflatten_list_val :
   forall el from to, 
-    map (fun '(x, y) => (rename_PID_val from to x, rename_PID_val from to y)) (deflatten_list el) =
-    deflatten_list (map (rename_PID_val from to) el).
+    map (fun '(x, y) => (renamePIDVal from to x, renamePIDVal from to y)) (deflatten_list el) =
+    deflatten_list (map (renamePIDVal from to) el).
 Proof.
   induction el using list_length_ind; destruct el; intros; simpl; auto.
   destruct el; auto. simpl.
   do 2 f_equal. rewrite H. reflexivity. slia.
 Qed.
 
-Proposition rename_PID_match_pattern :
+Proposition renamePID_match_pattern :
   forall p v vs', match_pattern p v = Some vs' ->
     forall from to,
-      match_pattern p (rename_PID_val from to v) = Some (map (rename_PID_val from to) vs').
+      match_pattern p (renamePIDVal from to v) = Some (map (renamePIDVal from to) vs').
 Proof.
   induction p using Pat_ind2
     with (Q := fun l => Forall (fun p => forall v vs', match_pattern p v = Some vs' ->
     forall from to,
-      match_pattern p (rename_PID_val from to v) = Some (map (rename_PID_val from to) vs')) l)
+      match_pattern p (renamePIDVal from to v) = Some (map (renamePIDVal from to) vs')) l)
       (R := fun l => Forall (PBoth (fun p => forall v vs', match_pattern p v = Some vs' ->
     forall from to,
-      match_pattern p (rename_PID_val from to v) = Some (map (rename_PID_val from to) vs'))) l); try destruct v; simpl; intros; try inv H; simpl; auto.
+      match_pattern p (renamePIDVal from to v) = Some (map (renamePIDVal from to) vs'))) l); try destruct v; simpl; intros; try inv H; simpl; auto.
   * break_match_hyp; inv H1; now simpl.
   * repeat break_match_hyp; try congruence. inv H1.
     eapply IHp1 in Heqo. eapply IHp2 in Heqo0. now rewrite Heqo, Heqo0, map_app.
@@ -465,28 +465,28 @@ Proof.
       apply IHIHp in Heqo1. rewrite Heqo1. now rewrite map_app, map_app.
 Qed.
 
-Proposition rename_PID_nomatch_pattern :
+Proposition renamePID_nomatch_pattern :
   forall p v, match_pattern p v = None ->
     forall from to,
-      match_pattern p (rename_PID_val from to v) = None.
+      match_pattern p (renamePIDVal from to v) = None.
 Proof.
   induction p using Pat_ind2
     with (Q := fun l => Forall (fun p => forall v, match_pattern p v = None ->
     forall from to,
-      match_pattern p (rename_PID_val from to v) = None) l)
+      match_pattern p (renamePIDVal from to v) = None) l)
       (R := fun l => Forall (PBoth (fun p => forall v, match_pattern p v = None ->
     forall from to,
-      match_pattern p (rename_PID_val from to v) = None)) l); try destruct v; simpl; intros; try now (inv H; simpl; auto).
+      match_pattern p (renamePIDVal from to v) = None)) l); try destruct v; simpl; intros; try now (inv H; simpl; auto).
   all: try now break_match_goal; auto; break_match_hyp; congruence.
   * repeat break_match_hyp; try congruence; inv H.
-    - eapply rename_PID_match_pattern in Heqo. eapply IHp2 in Heqo0.
+    - eapply renamePID_match_pattern in Heqo. eapply IHp2 in Heqo0.
       now rewrite Heqo, Heqo0.
     - eapply IHp1 in Heqo. now rewrite Heqo.
   * generalize dependent l0. induction IHp; intros.
     - destruct l0; now inv H.
     - destruct l0; inv H0. now simpl.
       simpl. break_match_hyp.
-      + eapply rename_PID_match_pattern in Heqo. rewrite Heqo. break_match_hyp. congruence.
+      + eapply renamePID_match_pattern in Heqo. rewrite Heqo. break_match_hyp. congruence.
         apply IHIHp in Heqo0. now rewrite Heqo0.
       + eapply H in Heqo. now rewrite Heqo.
   * generalize dependent l0. induction IHp; intros.
@@ -494,10 +494,10 @@ Proof.
     - destruct x; cbn in *. destruct l0; inv H0. now simpl. destruct H as [H_1 H_2].
       destruct p1. simpl in *.
       break_match_hyp. break_match_hyp. break_match_hyp. congruence.
-      + eapply rename_PID_match_pattern in Heqo. rewrite Heqo.
-        eapply rename_PID_match_pattern in Heqo0. rewrite Heqo0.
+      + eapply renamePID_match_pattern in Heqo. rewrite Heqo.
+        eapply renamePID_match_pattern in Heqo0. rewrite Heqo0.
         apply IHIHp in Heqo1. now rewrite Heqo1.
-      + eapply rename_PID_match_pattern in Heqo. rewrite Heqo.
+      + eapply renamePID_match_pattern in Heqo. rewrite Heqo.
         eapply H_2 in Heqo0. now rewrite Heqo0.
       + eapply H_1 in Heqo. now rewrite Heqo.
   * constructor; auto.
@@ -506,32 +506,32 @@ Proof.
   * constructor; auto.
 Qed.
 
-Corollary rename_PID_match_pattern_list :
+Corollary renamePID_match_pattern_list :
   forall lp vs vs', match_pattern_list lp vs = Some vs' ->
     forall from to,
-      match_pattern_list lp (map (rename_PID_val from to) vs) = Some (map (rename_PID_val from to) vs').
+      match_pattern_list lp (map (renamePIDVal from to) vs) = Some (map (renamePIDVal from to) vs').
 Proof.
   induction lp; destruct vs; simpl; intros; try congruence.
   * now inv H.
   * break_match_hyp. 2: congruence. break_match_hyp. 2: congruence.
-    eapply rename_PID_match_pattern in Heqo. rewrite Heqo. inv H.
+    eapply renamePID_match_pattern in Heqo. rewrite Heqo. inv H.
     eapply IHlp in Heqo0. rewrite Heqo0. now rewrite map_app.
 Qed.
 
-Corollary rename_PID_nomatch_pattern_list :
+Corollary renamePID_nomatch_pattern_list :
   forall lp vs, match_pattern_list lp vs = None ->
     forall from to,
-      match_pattern_list lp (map (rename_PID_val from to) vs) = None.
+      match_pattern_list lp (map (renamePIDVal from to) vs) = None.
 Proof.
   induction lp; destruct vs; simpl; intros; try congruence.
   break_match_hyp. break_match_hyp. congruence.
-  * eapply IHlp in Heqo0. eapply rename_PID_match_pattern in Heqo.
+  * eapply IHlp in Heqo0. eapply renamePID_match_pattern in Heqo.
     now rewrite Heqo, Heqo0.
-  * eapply rename_PID_nomatch_pattern in Heqo. now rewrite Heqo.
+  * eapply renamePID_nomatch_pattern in Heqo. now rewrite Heqo.
 Qed.
 
-Proposition rename_PID_Val_eqb :
-  forall v v' from to, v =ᵥ v' = rename_PID_val from to v =ᵥ rename_PID_val from to v'.
+Proposition renamePID_Val_eqb :
+  forall v v' from to, v =ᵥ v' = renamePIDVal from to v =ᵥ renamePIDVal from to v'.
 Proof.
   valinduction; try destruct v'; intros; simpl; auto.
   all: try now destruct Nat.eqb eqn:P.
@@ -544,16 +544,16 @@ Proof.
     - destruct x; simpl. destruct H, p. simpl in *. now erewrite IHIHv, H, H0.
 Qed.
 
-Proposition rename_PID_Val_ltb :
-  forall v v' from to, v <ᵥ v' = rename_PID_val from to v <ᵥ rename_PID_val from to v'.
+Proposition renamePID_Val_ltb :
+  forall v v' from to, v <ᵥ v' = renamePIDVal from to v <ᵥ renamePIDVal from to v'.
 Proof.
   valinduction; try destruct v'; intros; simpl; auto.
   all: try now destruct Nat.eqb eqn:P.
   * repeat break_match_goal; auto.
   * erewrite IHv1, IHv2.
-    break_match_goal; erewrite rename_PID_Val_eqb in Heqb; now rewrite Heqb.
+    break_match_goal; erewrite renamePID_Val_eqb in Heqb; now rewrite Heqb.
   * revert l0. induction IHv; destruct l0; simpl; auto.
-    break_match_goal; erewrite rename_PID_Val_eqb in Heqb; rewrite Heqb; specialize (IHIHv l0).
+    break_match_goal; erewrite renamePID_Val_eqb in Heqb; rewrite Heqb; specialize (IHIHv l0).
     all: repeat rewrite map_length in *.
     - rewrite Bool.orb_lazy_alt, Bool.andb_lazy_alt in IHIHv.
       repeat break_match_hyp; auto.
@@ -572,7 +572,7 @@ Proof.
         apply H.
   * revert l0. induction IHv; destruct l0; simpl; auto.
     destruct x, p, H.
-    break_match_goal; erewrite rename_PID_Val_eqb in Heqb; rewrite Heqb; specialize (IHIHv l0); simpl in *.
+    break_match_goal; erewrite renamePID_Val_eqb in Heqb; rewrite Heqb; specialize (IHIHv l0); simpl in *.
     all: repeat rewrite map_length in *.
     - rewrite Bool.orb_lazy_alt, Bool.andb_lazy_alt in IHIHv.
       repeat break_match_hyp; auto.
@@ -595,11 +595,11 @@ Proof.
         erewrite H, H0. admit. (* TODO Technical *)
 Admitted.
 
-Lemma rename_PID_make_val_map :
+Lemma renamePID_make_val_map :
   forall vs from to,
-  map (fun '(x, y) => (rename_PID_val from to x, rename_PID_val from to y))
+  map (fun '(x, y) => (renamePIDVal from to x, renamePIDVal from to y))
          (make_val_map vs) =
-  make_val_map (map (fun '(x, y) => (rename_PID_val from to x, rename_PID_val from to y))
+  make_val_map (map (fun '(x, y) => (renamePIDVal from to x, renamePIDVal from to y))
          vs).
 Proof.
   induction vs; intros; simpl; auto.
@@ -609,7 +609,7 @@ Proof.
   remember (make_val_map vs) as vl. clear Heqvl vs.
   revert v v0 from to.
   induction vl; intros; simpl; auto.
-  destruct a. erewrite (rename_PID_Val_eqb _ _ from to), (rename_PID_Val_ltb _ _ from to).
+  destruct a. erewrite (renamePID_Val_eqb _ _ from to), (renamePID_Val_ltb _ _ from to).
   repeat break_match_goal; simpl; eauto.
   now rewrite IHvl.
 Qed.
@@ -619,11 +619,11 @@ Ltac destruct_eqb_in_if EQ :=
   | [|- context G [if ?from =? ?p then _ else _]] => destruct (from =? p) eqn:EQ
   end.
 
-Lemma rename_PID_eval_arith :
+Lemma renamePID_eval_arith :
   forall m f vs r,
     eval_arith m f vs = r ->
     forall from to,
-      eval_arith m f (map (rename_PID_val from to) vs) = rename_PID_red from to r.
+      eval_arith m f (map (renamePIDVal from to) vs) = renamePIDRed from to r.
 Proof.
   intros. unfold eval_arith in *. break_match_goal; inv H.
   all: destruct vs; simpl; try reflexivity.
@@ -639,63 +639,63 @@ Proof.
   all: destruct x0; try reflexivity.
 Qed.
 
-Lemma rename_PID_eval_logical :
+Lemma renamePID_eval_logical :
   forall m f vs r,
     eval_logical m f vs = r ->
     forall from to,
-      eval_logical m f (map (rename_PID_val from to) vs) = rename_PID_red from to r.
+      eval_logical m f (map (renamePIDVal from to) vs) = renamePIDRed from to r.
 Proof.
   intros. unfold eval_logical in *. break_match_goal; inv H; try reflexivity; clear Heqb.
   all: destruct vs; simpl; try reflexivity.
   all: destruct vs; simpl; try reflexivity.
   all: try destruct vs; simpl; try reflexivity.
   all: repeat break_match_hyp.
-  all: erewrite rename_PID_Val_eqb in Heqb;
-       try erewrite rename_PID_Val_eqb in Heqb0;
-       try erewrite rename_PID_Val_eqb in Heqb1.
+  all: erewrite renamePID_Val_eqb in Heqb;
+       try erewrite renamePID_Val_eqb in Heqb0;
+       try erewrite renamePID_Val_eqb in Heqb1.
   all: simpl in *; try rewrite Heqb;
                    try rewrite Heqb0;
                    try rewrite Heqb1;
                    try reflexivity.
-  all: erewrite rename_PID_Val_eqb in Heqb2; rewrite Heqb2; try reflexivity.
+  all: erewrite renamePID_Val_eqb in Heqb2; rewrite Heqb2; try reflexivity.
 Qed.
 
-Lemma rename_PID_eval_equality :
+Lemma renamePID_eval_equality :
   forall m f vs r,
     eval_equality m f vs = r ->
     forall from to,
-      eval_equality m f (map (rename_PID_val from to) vs) = rename_PID_red from to r.
+      eval_equality m f (map (renamePIDVal from to) vs) = renamePIDRed from to r.
 Proof.
   intros. unfold eval_equality in *. break_match_goal; inv H; try reflexivity; clear Heqb.
   all: destruct vs; simpl; try reflexivity.
   all: destruct vs; simpl; try reflexivity.
   all: destruct vs; simpl; try reflexivity.
-  all: destruct Val_eqb eqn:P; erewrite rename_PID_Val_eqb in P; rewrite P.
+  all: destruct Val_eqb eqn:P; erewrite renamePID_Val_eqb in P; rewrite P.
   all: reflexivity.
 Qed.
 
-Lemma rename_PID_eval_cmp :
+Lemma renamePID_eval_cmp :
   forall m f vs r,
     eval_cmp m f vs = r ->
     forall from to,
-      eval_cmp m f (map (rename_PID_val from to) vs) = rename_PID_red from to r.
+      eval_cmp m f (map (renamePIDVal from to) vs) = renamePIDRed from to r.
 Proof.
   intros. unfold eval_cmp in *. break_match_goal; inv H; try reflexivity; clear Heqb.
   all: destruct vs; simpl; try reflexivity.
   all: destruct vs; simpl; try reflexivity.
   all: destruct vs; simpl; try reflexivity.
-  all: destruct Val_ltb eqn:P; erewrite rename_PID_Val_ltb in P; rewrite P.
+  all: destruct Val_ltb eqn:P; erewrite renamePID_Val_ltb in P; rewrite P.
   all: try reflexivity.
   all: simpl in *.
-  all: destruct Val_eqb eqn:P0; erewrite rename_PID_Val_eqb in P0; rewrite P0.
+  all: destruct Val_eqb eqn:P0; erewrite renamePID_Val_eqb in P0; rewrite P0.
   all: try reflexivity.
 Qed.
 
-Lemma rename_PID_eval_hd_tl :
+Lemma renamePID_eval_hd_tl :
   forall m f vs r,
     eval_hd_tl m f vs = r ->
     forall from to,
-      eval_hd_tl m f (map (rename_PID_val from to) vs) = rename_PID_red from to r.
+      eval_hd_tl m f (map (renamePIDVal from to) vs) = renamePIDRed from to r.
 Proof.
   intros. unfold eval_hd_tl in *. break_match_goal; inv H; try reflexivity; clear Heqb.
   all: destruct vs; simpl; try reflexivity.
@@ -703,11 +703,11 @@ Proof.
   all: destruct v; try reflexivity; simpl; destruct Nat.eqb; try reflexivity.
 Qed.
 
-Lemma rename_PID_eval_check :
+Lemma renamePID_eval_check :
   forall m f vs r,
     eval_check m f vs = r ->
     forall from to,
-      eval_check m f (map (rename_PID_val from to) vs) = rename_PID_red from to r.
+      eval_check m f (map (renamePIDVal from to) vs) = renamePIDRed from to r.
 Proof.
   intros. unfold eval_check in *. break_match_goal; inv H; try reflexivity; clear Heqb.
   all: destruct vs; simpl; try reflexivity.
@@ -719,11 +719,11 @@ Proof.
   destruct string_dec; reflexivity.
 Qed.
 
-Lemma rename_PID_eval_funinfo :
+Lemma renamePID_eval_funinfo :
   forall vs r,
     eval_funinfo vs = r ->
     forall from to,
-      eval_funinfo (map (rename_PID_val from to) vs) = rename_PID_red from to r.
+      eval_funinfo (map (renamePIDVal from to) vs) = renamePIDRed from to r.
 Proof.
   intros. unfold eval_funinfo in *.
   all: destruct vs; simpl; try reflexivity.
@@ -735,16 +735,16 @@ Proof.
     all: try destruct (Nat.eqb from p) eqn:P; try now inversion H.
     inv H; cbn; destruct Nat.eqb; cbn; try reflexivity; try congruence.
     inv H; cbn; destruct Nat.eqb; cbn; try reflexivity; try congruence.
-    break_match_hyp; erewrite rename_PID_Val_eqb in Heqb; rewrite Heqb.
+    break_match_hyp; erewrite renamePID_Val_eqb in Heqb; rewrite Heqb.
     now inv H.
     now inv H.
 Qed.
 
-Lemma rename_PID_eval_transform_list :
+Lemma renamePID_eval_transform_list :
   forall m f vs r,
     eval_transform_list m f vs = r ->
     forall from to,
-      eval_transform_list m f (map (rename_PID_val from to) vs) = rename_PID_red from to r.
+      eval_transform_list m f (map (renamePIDVal from to) vs) = renamePIDRed from to r.
 Proof.
   intros. unfold eval_transform_list in *. break_match_goal; inv H; try reflexivity; clear Heqb.
   all: destruct vs; simpl; try reflexivity.
@@ -764,11 +764,11 @@ Proof.
   }
 Admitted.
 
-Lemma rename_PID_eval_elem_tuple :
+Lemma renamePID_eval_elem_tuple :
   forall m f vs r,
     eval_elem_tuple m f vs = r ->
     forall from to,
-      eval_elem_tuple m f (map (rename_PID_val from to) vs) = rename_PID_red from to r.
+      eval_elem_tuple m f (map (renamePIDVal from to) vs) = renamePIDRed from to r.
 Proof.
   intros. unfold eval_elem_tuple in *.
   break_match_goal; inv H; try reflexivity; clear Heqb.
@@ -788,11 +788,11 @@ Proof.
   * rewrite replace_nth_error_map. now destruct replace_nth_error.
 Qed.
 
-Lemma rename_PID_eval_list_tuple :
+Lemma renamePID_eval_list_tuple :
   forall m f vs r,
     eval_list_tuple m f vs = r ->
     forall from to,
-      eval_list_tuple m f (map (rename_PID_val from to) vs) = rename_PID_red from to r.
+      eval_list_tuple m f (map (renamePIDVal from to) vs) = renamePIDRed from to r.
 Proof.
   intros. unfold eval_list_tuple in *.
   break_match_goal; inv H; try reflexivity; clear Heqb.
@@ -814,11 +814,11 @@ Proof.
     Transparent transform_list.
 Qed.
 
-Lemma rename_PID_eval_length :
+Lemma renamePID_eval_length :
   forall vs r,
     eval_length vs = r ->
     forall from to,
-      eval_length (map (rename_PID_val from to) vs) = rename_PID_red from to r.
+      eval_length (map (renamePIDVal from to) vs) = renamePIDRed from to r.
 Proof.
   intros. unfold eval_length in *.
   rewrite <- H. clear H.
@@ -832,11 +832,11 @@ Proof.
   * break_match_hyp; inv H0. reflexivity.
 Qed.
 
-Lemma rename_PID_eval_tuple_size :
+Lemma renamePID_eval_tuple_size :
   forall vs r,
     eval_tuple_size vs = r ->
     forall from to,
-      eval_tuple_size (map (rename_PID_val from to) vs) = rename_PID_red from to r.
+      eval_tuple_size (map (renamePIDVal from to) vs) = renamePIDRed from to r.
 Proof.
   intros. unfold eval_tuple_size in *.
   rewrite <- H. clear H.
@@ -848,12 +848,12 @@ Proof.
   all: now destruct Nat.eqb.
 Qed.
 
-Lemma rename_PID_eval_io :
+Lemma renamePID_eval_io :
   forall m f vs eff r eff',
     eval_io m f vs eff = (r, eff') ->
     forall from to,
-      eval_io m f (map (rename_PID_val from to) vs) (map (fun '(a, b) => (a, map (rename_PID_val from to) b)) eff) =
-        (rename_PID_red from to r, map (fun '(a, b) => (a, map (rename_PID_val from to) b)) eff').
+      eval_io m f (map (renamePIDVal from to) vs) (map (fun '(a, b) => (a, map (renamePIDVal from to) b)) eff) =
+        (renamePIDRed from to r, map (fun '(a, b) => (a, map (renamePIDVal from to) b)) eff').
 Proof.
   intros. unfold eval_io in *. break_match_goal; inv H; clear Heqb; try reflexivity.
   all: rewrite map_length.
@@ -864,11 +864,11 @@ Proof.
   all: simpl; rewrite map_app; reflexivity.
 Qed.
 
-Lemma rename_PID_eval_concurrent :
+Lemma renamePID_eval_concurrent :
   forall m f vs class reas det,
     eval_concurrent m f vs = Some (class, reas, det) ->
     forall from to,
-      eval_concurrent m f (map (rename_PID_val from to) vs) = Some (class, rename_PID_val from to reas, rename_PID_val from to det).
+      eval_concurrent m f (map (renamePIDVal from to) vs) = Some (class, renamePIDVal from to reas, renamePIDVal from to det).
 Proof.
   intros. unfold eval_concurrent in *. break_match_goal; inv H; clear Heqb; try reflexivity.
   all: destruct vs; inv H1; simpl; try reflexivity.
@@ -876,11 +876,11 @@ Proof.
 Qed.
 
 
-Lemma rename_PID_eval_error :
+Lemma renamePID_eval_error :
   forall m f vs class reas det,
     eval_error m f vs = Some (class, reas, det) ->
     forall from to,
-      eval_error m f (map (rename_PID_val from to) vs) = Some (class, rename_PID_val from to reas, rename_PID_val from to det).
+      eval_error m f (map (renamePIDVal from to) vs) = Some (class, renamePIDVal from to reas, renamePIDVal from to det).
 Proof.
   intros. unfold eval_error in *. break_match_goal; inv H; clear Heqb; try reflexivity.
   all: destruct vs; inv H1; simpl; try reflexivity.
@@ -889,41 +889,41 @@ Proof.
   all: destruct vs; inv H0; simpl; try reflexivity.
 Qed.
 
-Proposition rename_PID_eval :
+Proposition renamePID_eval :
   forall m f vs eff r eff',
     eval m f vs eff = Some (r, eff') ->
     forall from to,
-      eval m f (map (rename_PID_val from to) vs) (map (fun '(a, b) => (a, map (rename_PID_val from to) b)) eff) =
-        Some (rename_PID_red from to r, map (fun '(a, b) => (a, map (rename_PID_val from to) b)) eff').
+      eval m f (map (renamePIDVal from to) vs) (map (fun '(a, b) => (a, map (renamePIDVal from to) b)) eff) =
+        Some (renamePIDRed from to r, map (fun '(a, b) => (a, map (renamePIDVal from to) b)) eff').
 Proof.
   intros. unfold eval in *.
   break_match_hyp; try rewrite Heqb in *; inv H.
   all:
-    try (erewrite rename_PID_eval_arith; reflexivity);
-    try (erewrite rename_PID_eval_logical; reflexivity);
-    try (erewrite rename_PID_eval_equality; reflexivity);
-    try (erewrite rename_PID_eval_cmp; reflexivity);
-    try (erewrite rename_PID_eval_hd_tl; reflexivity);
-    try (erewrite rename_PID_eval_funinfo; reflexivity);
-    try (erewrite rename_PID_eval_length; reflexivity);
-    try (erewrite rename_PID_eval_elem_tuple; reflexivity);
-    try (erewrite rename_PID_eval_transform_list; reflexivity);
-    try (erewrite rename_PID_eval_list_tuple; reflexivity);
-    try (erewrite rename_PID_eval_tuple_size; reflexivity);
-    try (erewrite rename_PID_eval_check; reflexivity).
-  1-2: erewrite rename_PID_eval_io; try eassumption; reflexivity.
+    try (erewrite renamePID_eval_arith; reflexivity);
+    try (erewrite renamePID_eval_logical; reflexivity);
+    try (erewrite renamePID_eval_equality; reflexivity);
+    try (erewrite renamePID_eval_cmp; reflexivity);
+    try (erewrite renamePID_eval_hd_tl; reflexivity);
+    try (erewrite renamePID_eval_funinfo; reflexivity);
+    try (erewrite renamePID_eval_length; reflexivity);
+    try (erewrite renamePID_eval_elem_tuple; reflexivity);
+    try (erewrite renamePID_eval_transform_list; reflexivity);
+    try (erewrite renamePID_eval_list_tuple; reflexivity);
+    try (erewrite renamePID_eval_tuple_size; reflexivity);
+    try (erewrite renamePID_eval_check; reflexivity).
+  1-2: erewrite renamePID_eval_io; try eassumption; reflexivity.
   1-3: break_match_hyp; try congruence; destruct e, p;
-       eapply rename_PID_eval_error in Heqo; rewrite Heqo; inv H1; reflexivity.
+       eapply renamePID_eval_error in Heqo; rewrite Heqo; inv H1; reflexivity.
   1-6: break_match_hyp; try congruence; destruct e, p;
-       eapply rename_PID_eval_concurrent in Heqo; rewrite Heqo; inv H1; reflexivity.
+       eapply renamePID_eval_concurrent in Heqo; rewrite Heqo; inv H1; reflexivity.
   reflexivity.
 Qed.
 
-Proposition rename_PID_primop_eval :
+Proposition renamePID_primop_eval :
   forall f vs eff r eff',
     primop_eval f vs eff = Some (r, eff') ->
     forall from to,
-      primop_eval f (map (rename_PID_val from to) vs) (map (fun '(a, b) => (a, map (rename_PID_val from to) b)) eff) = Some (rename_PID_red from to r, map (fun '(a, b) => (a, map (rename_PID_val from to) b)) eff').
+      primop_eval f (map (renamePIDVal from to) vs) (map (fun '(a, b) => (a, map (renamePIDVal from to) b)) eff) = Some (renamePIDRed from to r, map (fun '(a, b) => (a, map (renamePIDVal from to) b)) eff').
 Proof.
   intros. destruct (convert_primop_to_code f) eqn:EQ;
   unfold primop_eval in *; rewrite EQ in *.
@@ -936,76 +936,184 @@ Proof.
   1: now inv H.
 Qed.
 
-Corollary rename_PID_create_result :
+Corollary renamePID_create_result :
   forall vs ident eff r eff',
     create_result ident vs eff = Some (r, eff') ->
-    forall from to, create_result (rename_PID_frameId from to ident)
-                                  (map (rename_PID_val from to) vs) (map (fun '(a, b) => (a, map (rename_PID_val from to) b)) eff) =
-                                  Some (rename_PID_red from to r, map (fun '(a, b) => (a, map (rename_PID_val from to) b)) eff').
+    forall from to, create_result (renamePIDFrameId from to ident)
+                                  (map (renamePIDVal from to) vs) (map (fun '(a, b) => (a, map (renamePIDVal from to) b)) eff) =
+                                  Some (renamePIDRed from to r, map (fun '(a, b) => (a, map (renamePIDVal from to) b)) eff').
 Proof.
   intros. destruct ident; simpl in *.
   * now inv H.
   * now inv H.
   * inv H. cbn.
-    now rewrite <- rename_subst_deflatten_list_val, rename_PID_make_val_map.
+    now rewrite <- rename_subst_deflatten_list_val, renamePID_make_val_map.
   * destruct m, f; simpl in *; inv H; auto.
     all: try destruct l; try destruct l0; try inv H1; auto.
     2-14: destruct (from =? p) eqn:P; cbn; now try rewrite P.
-    eapply rename_PID_eval in H0. simpl in H0. exact H0.
-  * eapply rename_PID_primop_eval in H. exact H.
+    eapply renamePID_eval in H0. simpl in H0. exact H0.
+  * eapply renamePID_primop_eval in H. exact H.
   * rewrite map_length.
     destruct v; simpl. all: try now inv H.
     - destruct Nat.eqb eqn:P; inv H; cbn; now rewrite P.
     - break_match_hyp; try now inv H.
-      inv H. simpl. rewrite split_rename_PID_subst_exp, rename_PID_subst_list_subst.
+      inv H. simpl. rewrite split_renamePID_subst_exp, renamePID_subst_list_subst.
       unfold convert_to_closlist. repeat f_equal.
       rewrite map_map, map_app. f_equal. rewrite map_map.
       f_equal. extensionality x. destruct x, p. cbn. f_equal.
 Qed.
 
-Theorem rename_PID_is_preserved :
+Theorem renamePID_is_preserved :
   forall fs r fs' r', ⟨fs, r⟩ --> ⟨fs', r'⟩ ->
     forall from to,
-      ⟨rename_PID_stack from to fs, rename_PID_red from to r⟩ -->
-      ⟨rename_PID_stack from to fs', rename_PID_red from to r'⟩.
+      ⟨renamePIDStack from to fs, renamePIDRed from to r⟩ -->
+      ⟨renamePIDStack from to fs', renamePIDRed from to r'⟩.
 Proof.
   intros. inv H; cbn; try now constructor.
-  * constructor. now apply rename_PID_preserves_scope.
+  * constructor. now apply renamePID_preserves_scope.
   * rewrite map_app. constructor.
   * constructor. destruct ident; cbn; congruence.
   * econstructor.
     - destruct ident; cbn; congruence.
-    - eapply eq_sym, rename_PID_create_result in H1. symmetry. eassumption.
+    - eapply eq_sym, renamePID_create_result in H1. symmetry. eassumption.
   * econstructor.
-    - replace (map (rename_PID_val from to) vl ++ [rename_PID_val from to v]) with
-              (map (rename_PID_val from to) (vl ++ [v])) by now rewrite map_app.
-      eapply eq_sym, rename_PID_create_result in H0. symmetry. eassumption.
+    - replace (map (renamePIDVal from to) vl ++ [renamePIDVal from to v]) with
+              (map (renamePIDVal from to) (vl ++ [v])) by now rewrite map_app.
+      eapply eq_sym, renamePID_create_result in H0. symmetry. eassumption.
   * rewrite rename_subst_flatten_list. constructor.
-  * rewrite split_rename_PID_subst_exp,
-            rename_PID_subst_list_subst,
-            rename_PID_subst_id.
+  * rewrite split_renamePID_subst_exp,
+            renamePID_subst_list_subst,
+            renamePID_subst_id.
     constructor. now rewrite map_length.
-  * repeat rewrite split_rename_PID_subst_exp,
-                   rename_PID_subst_list_subst,
-                   rename_PID_subst_id.
-    constructor. now apply rename_PID_match_pattern_list.
-  * econstructor. now apply rename_PID_nomatch_pattern_list.
-  * rewrite split_rename_PID_subst_exp,
-            rename_PID_subst_list_subst,
-            rename_PID_subst_id.
+  * repeat rewrite split_renamePID_subst_exp,
+                   renamePID_subst_list_subst,
+                   renamePID_subst_id.
+    constructor. now apply renamePID_match_pattern_list.
+  * econstructor. now apply renamePID_nomatch_pattern_list.
+  * rewrite split_renamePID_subst_exp,
+            renamePID_subst_list_subst,
+            renamePID_subst_id.
     constructor.
     unfold convert_to_closlist. repeat rewrite map_map. f_equal.
     extensionality x. destruct x. simpl. rewrite map_map. do 2 f_equal.
     extensionality x. now destruct x.
-  * rewrite split_rename_PID_subst_exp,
-            rename_PID_subst_list_subst,
-            rename_PID_subst_id.
+  * rewrite split_renamePID_subst_exp,
+            renamePID_subst_list_subst,
+            renamePID_subst_id.
     constructor. now rewrite map_length.
-  * rewrite split_rename_PID_subst_exp.
-    pose proof (rename_PID_subst_list_subst [exclass_to_value class; reason; details]).
+  * rewrite split_renamePID_subst_exp.
+    pose proof (renamePID_subst_list_subst [exclass_to_value class; reason; details]).
     simpl in H. rewrite H.
     destruct class; cbn; constructor.
   * destruct exc, p. constructor.
     destruct F; auto.
 Qed.
 
+(* NOTE: instead of fold_right, Exists would be better, but Coq cannot guess the
+   decreasing argument that way. *)
+Fixpoint isUsedPIDExp (from : PID) (e : Exp) : Prop :=
+match e with
+ | VVal e => isUsedPIDVal from e
+ | EExp e => isUsedPIDNVal from e
+end
+with isUsedPIDVal (from : PID) (v : Val) : Prop :=
+match v with
+ | VNil => False
+ | VLit l => False
+ | VPid p => from = p
+ | VCons hd tl => isUsedPIDVal from hd \/ isUsedPIDVal from tl
+ | VTuple l => fold_right (fun x acc => isUsedPIDVal from x \/ acc) False l
+ | VMap l => fold_right (fun '(x, y) acc => isUsedPIDVal from x \/ isUsedPIDVal from y \/ acc) False l
+ | VVar n => False
+ | VFunId n => False
+ | VClos ext id params e => fold_right (fun '(_, _, x) acc => isUsedPIDExp from x \/ acc) False ext \/ isUsedPIDExp from e
+end
+with isUsedPIDNVal (from : PID) (n : NonVal) : Prop :=
+match n with
+ | EFun vl e => isUsedPIDExp from e
+ | EValues el => fold_right (fun x acc => isUsedPIDExp from x \/ acc) False el
+ | ECons hd tl => isUsedPIDExp from hd \/ isUsedPIDExp from tl
+ | ETuple l => fold_right (fun x acc => isUsedPIDExp from x \/ acc) False l
+ | EMap l => fold_right (fun '(x, y) acc => isUsedPIDExp from x \/ isUsedPIDExp from y \/ acc) False l
+ | ECall m f l => isUsedPIDExp from m \/ isUsedPIDExp from f \/ fold_right (fun x acc => isUsedPIDExp from x \/ acc) False l
+ | EPrimOp f l => fold_right (fun x acc => isUsedPIDExp from x \/ acc) False l
+ | EApp exp l => (isUsedPIDExp from exp) \/ fold_right (fun x acc => isUsedPIDExp from x \/ acc) False l
+ | ECase e l => (isUsedPIDExp from e) \/ fold_right (fun '(_, g, e) acc => isUsedPIDExp from g \/ isUsedPIDExp from e \/ acc) False l
+ | ELet l e1 e2 => isUsedPIDExp from e1 \/ isUsedPIDExp from e2
+ | ESeq e1 e2 => isUsedPIDExp from e1 \/ isUsedPIDExp from e2
+ | ELetRec l e => (isUsedPIDExp from e) \/ fold_right (fun '(_, e) acc => isUsedPIDExp from e \/ acc) False l
+ | ETry e1 vl1 e2 vl2 e3 => isUsedPIDExp from e1 \/ isUsedPIDExp from e2 \/ isUsedPIDExp from e3
+end.
+
+Definition isUsedPIDRed (from : PID) (r : Redex) : Prop :=
+match r with
+ | RExp e => isUsedPIDExp from e
+ | RValSeq vs => fold_right (fun x acc => isUsedPIDVal from x \/ acc) False vs
+ | RExc (class, reas, det) => isUsedPIDVal from reas \/ isUsedPIDVal from det
+ | RBox => False
+end.
+
+
+Definition isUsedPIDFrameId (from : PID) (f : FrameIdent) : Prop :=
+match f with
+ | ICall m f => isUsedPIDVal from m \/ isUsedPIDVal from f
+ | IApp v => isUsedPIDVal from v
+ | _ => False
+end.
+
+Definition isUsedPIDFrame (from : PID) (f : Frame) : Prop :=
+match f with
+ | FCons1 hd => isUsedPIDExp from hd
+ | FCons2 tl => isUsedPIDVal from tl
+ | FParams ident vl el =>
+     (isUsedPIDFrameId from ident) \/
+     fold_right (fun x acc => isUsedPIDExp from x \/ acc) False el \/
+     fold_right (fun x acc => isUsedPIDVal from x \/ acc) False vl
+ | FApp1 l => fold_right (fun x acc => isUsedPIDExp from x \/ acc) False l
+ | FCallMod f l => (isUsedPIDExp from f) \/ fold_right (fun x acc => isUsedPIDExp from x \/ acc) False l
+ | FCallFun m l => (isUsedPIDVal from m) \/ fold_right (fun x acc => isUsedPIDExp from x \/ acc) False l
+ | FCase1 l => fold_right (fun '(_, g, e) acc => isUsedPIDExp from g \/ isUsedPIDExp from e \/ acc) False l
+ | FCase2 lv ex le =>
+   (isUsedPIDExp from ex) \/
+   fold_right (fun x acc => isUsedPIDVal from x \/ acc) False lv \/
+   fold_right (fun '(_, g, e) acc => isUsedPIDExp from g \/ isUsedPIDExp from e \/ acc) False le
+ | FLet l e => isUsedPIDExp from e
+ | FSeq e => isUsedPIDExp from e
+ | FTry vl1 e2 vl2 e3 => isUsedPIDExp from e2 \/  isUsedPIDExp from e3
+end.
+
+Definition isUsedPIDStack (from : PID) (fs : FrameStack) : Prop :=
+  fold_right (fun x acc => isUsedPIDFrame from x \/ acc) False fs.
+
+Local Theorem isNotUsed_renamePID_ind :
+  (forall e from to, ~isUsedPIDExp from e -> renamePID from to e = e) /\
+  (forall e from to, ~isUsedPIDNVal from e -> renamePIDNVal from to e = e) /\
+  (forall e from to, ~isUsedPIDVal from e -> renamePIDVal from to e = e).
+Proof.
+  apply Exp_ind with
+    (QV := fun l => Forall (fun e => forall from to, ~isUsedPIDVal from e -> renamePIDVal from to e = e) l)
+    (Q := fun l => Forall (fun e => forall from to, ~isUsedPIDExp from e -> renamePID from to e = e) l)
+    (RV := fun l => Forall (fun '(e1, e2) => forall from to,
+        (~isUsedPIDVal from e1 -> renamePIDVal from to e1 = e1) /\
+        (~isUsedPIDVal from e2 -> renamePIDVal from to e2 = e2)) l)
+    (R := fun l => Forall (fun '(e1, e2) => forall from to,
+        (~isUsedPIDExp from e1 -> renamePID from to e1 = e1) /\
+        (~isUsedPIDExp from e2 -> renamePID from to e1 = e2)) l)
+    (W := fun l => Forall (fun '(p, g, e) => forall from to,
+       (~isUsedPIDExp from g -> renamePID from to e = g) /\
+       (~isUsedPIDExp from e -> renamePID from to e = e)) l)
+    (Z := fun l => Forall (fun '(n, e) => forall from to, ~isUsedPIDExp from e -> renamePID from to e = e) l)
+   (VV := fun l => Forall
+      (fun '(id, vl, e) => forall from to, ~isUsedPIDExp from e -> renamePID from to e = e) l); intros; simpl; try reflexivity.
+  all: try now intuition.
+  all: try rewrite H; try rewrite H0; auto; try firstorder.
+  * simpl in H. break_match_goal. now apply Nat.eqb_eq in Heqb. reflexivity.
+  * f_equal. rewrite <- (map_id l) at 2. apply map_ext_in.
+    rewrite Forall_forall in H. intros. eapply H in H1 as H1'. now erewrite H1'.
+    simpl in H0. rewrite <- Exists_fold_right, Exists_exists in H0. firstorder.
+  * f_equal. rewrite <- (map_id l) at 2. apply map_ext_in.
+    rewrite Forall_forall in H. intros. eapply H in H1 as H1'. destruct a.
+    erewrite (proj1 (H1' _ _)). erewrite (proj2 (H1' _ _)). reflexivity.
+    - simpl in H0.
+      rewrite <- Exists_fold_right with (P := fun x => ), Exists_exists in H0. firstorder.
+Qed.
